def: completeness of SKI

Rz/Algebra/PCA.lean
@@ -31,8 +31,6 @@ syntax term " ⊢ " magma " ⇓ " term:40 : term
 syntax term " ⊢ " magma " ≤ " term:max " ⊢ " withPosition(magma) : term
 syntax term " ⊢ " magma " ≃ " term:max " ⊢ " withPosition(magma) : term
 
--- ρ₁ ⊢ e₁ ≤ ρ₂ ⊢ e₂
-
 macro_rules
 | `($ρ:term ⊢ $e:magma ↑) => `(HasEval.Undefined $ρ («magma» $e))
 | `($ρ:term ⊢ $e:magma ↓) => `(HasEval.Defined $ρ («magma» $e))
@@ -43,20 +41,99 @@ macro_rules
 /-- Partial Applicative Structures. -/
 class PAS (α : Type u) extends HasEval α where
   /-- The evaluation relation is functional. -/
-  eval_functional : (ρ : Bwd α) → (e : FreeMagma α) → (a a' : α) → ρ ⊢ e ⇓ a → ρ ⊢ e ⇓ a' → a = a'
-  var_eval : (ρ : Bwd α) → (x : Fin ρ.length) → ρ ⊢ $(FreeMagma.var x) ⇓ ρ.get x
-  var_oob : (ρ : Bwd α) → (x : Nat) → ρ.length ≤ x → ρ ⊢ $(FreeMagma.var x) ↑
+  eval_functional : {ρ : Bwd α} → {e : FreeMagma α} → {a a' : α} → ρ ⊢ e ⇓ a → ρ ⊢ e ⇓ a' → a = a'
+  /-- Looking up the 0th variable resolves to the final element of the environment. -/
+  var_zero_eval : (ρ : Bwd α) → (a : α) → (ρ :# a) ⊢ $(FreeMagma.var 0) ⇓ a
+  /-- Resolving a successor variable requires us to look up in the tail of the environment. -/
+  var_succ_eval : (ρ : Bwd α) → (a : α) → (n : Nat) → (ρ :# a) ⊢ `(n+1) ≃ ρ ⊢ `(n)
+  /-- Resolving an out-of-bounds variable diverges. -/
+  var_zero_diverge : (n : Nat) → (Bwd.nil : Bwd α) ⊢ `(n+1) ↑
+  /-- Constants reduce to themselves. -/
   const_eval : (ρ : Bwd α) → (a : α) → ρ ⊢ a ⇓ a
-  ap_eval : {ρ : Bwd α} → {e₁ e₂ : FreeMagma α} → {a₁ a₂ : α} → ρ ⊢ e₁ ⇓ a₁ → ρ ⊢ e₂ ⇓ a₂ → ρ ⊢ e₁ e₂ ≃ ρ ⊢ a₁ a₂
+  ap_eval : {ρ₁ ρ₂ : Bwd α} → {e₁ e₂ : FreeMagma α} → {a₁ a₂ : α} → ρ₁ ⊢ e₁ ⇓ a₁ → ρ₁ ⊢ e₂ ⇓ a₂ → ρ₁ ⊢ e₁ e₂ ≃ ρ₂ ⊢ a₁ a₂
   ap_left_defined : {ρ : Bwd α} → {e₁ e₂ : FreeMagma α} → ρ ⊢ e₁ e₂ ↓ → ρ ⊢ e₁ ↓
   ap_right_defined : {ρ : Bwd α} → {e₁ e₂ : FreeMagma α} → ρ ⊢ e₁ e₂ ↓ → ρ ⊢ e₂ ↓
+
+/-!
+## Variable Lemmas
+-/
+
+/-- Variant of `var_succ_eval` that uses `Nat.pred`. -/
+theorem PAS.var_pred_eval_ne_zero
+  [PAS α]
+  (ρ : Bwd α) (a : α)
+  (n : Nat) (h : n ≠ 0)
+  : (ρ :# a) ⊢ `(n) ≃ ρ ⊢ `(n.pred) := by
+  match n with
+  | 0 => contradiction
+  | n+1 => apply PAS.var_succ_eval
+
+/-- -/
+theorem PAS.var_get_eval
+  [PAS α]
+  (ρ : Bwd α) (x : Fin ρ.length)
+  : ρ ⊢ `(x) ⇓ ρ.get x := by
+  match ρ with
+  | .nil =>
+    have : x.val < 0 := x.is_lt
+    contradiction
+  | .snoc ρ a =>
+    if h : x = 0 then
+      simp [h]
+      apply PAS.var_zero_eval
+    else
+      -- apply (PAS.var_pred_eval_ne_zero ρ a x h).2
+      sorry
+      -- rw [Bwd.get_snoc_pred_ne_zero ρ a x h]
+      -- apply PAS.var_get_eval
+
+/-!
+## Evaluation Lemmas
+-/
 
 theorem PAS.const_eval_eq
   [PAS α]
   (ρ : Bwd α)
   (a a' : α) (a_eval : ρ ⊢ a ⇓ a')
   : a = a' :=
-    eval_functional ρ (.const a) a a' (const_eval ρ a) a_eval
+    eval_functional (const_eval ρ a) a_eval
+
+/-- Evaluation of constants is invariant under environments. -/
+theorem PAS.const_eval_stable
+  [PAS α]
+  (ρ₁ ρ₂ : Bwd α)
+  (a a' : α) (a_eval : ρ₁ ⊢ a ⇓ a')
+  : ρ₂ ⊢ a ⇓ a' := by
+    rw [PAS.const_eval_eq ρ₁ a a' a_eval]
+    apply PAS.const_eval
+
+theorem PAS.closed_eval_stable
+  [PAS α]
+  (ρ₁ ρ₂ : Bwd α)
+  (e : FreeMagma α) (a : α)
+  (closed : e.fv = 0)
+  (a_eval : ρ₁ ⊢ e ⇓ a)
+  : ρ₂ ⊢ e ⇓ a := by
+    match e with
+    | .var _ => contradiction
+    | .const b =>
+       apply PAS.const_eval_stable
+       exact a_eval
+    | .ap e₁ e₂ =>
+      have ⟨ a₁ , a₁_eval_ρ₁ ⟩ := ap_left_defined ⟨ a , a_eval ⟩
+      have ⟨ a₂ , a₂_eval_ρ₁ ⟩ := ap_right_defined ⟨ a , a_eval ⟩
+      have ⟨ e₁_closed , e₂_closed ⟩ := FreeMagma.ap_closed_closed closed
+      have a₁_eval_ρ₂ : ρ₂ ⊢ e₁ ⇓ a₁ := by
+        apply PAS.closed_eval_stable
+        · exact e₁_closed
+        · exact a₁_eval_ρ₁
+      have a₂_eval_ρ₂ : ρ₂ ⊢ e₂ ⇓ a₂ := by
+        apply PAS.closed_eval_stable
+        · exact e₂_closed
+        · exact a₂_eval_ρ₁
+      apply (PAS.ap_eval a₁_eval_ρ₂ a₂_eval_ρ₂).2
+      apply (PAS.ap_eval (ρ₂ := ρ₂) a₁_eval_ρ₁ a₂_eval_ρ₁).1
+      · exact a_eval
 
 theorem PAS.const_defined [PAS α] (ρ : Bwd α) (a : α) : ρ ⊢ a ↓ :=
   ⟨ a , PAS.const_eval ρ a ⟩
@@ -89,9 +166,9 @@ class SKI (α : Type u) extends PAS α where
   i : α
   s_defined_2 : {ρ : Bwd α} → {e₁ e₂ : FreeMagma α} → ρ ⊢ e₁ ↓ → ρ ⊢ e₂ ↓ → ρ ⊢ s e₁ e₂ ↓
   k_defined : {ρ : Bwd α} → {e : FreeMagma α} → ρ ⊢ e ↓ → ρ ⊢ k e ↓
-  s_eval : (ρ : Bwd α) → (e₁ e₂ e₃ : FreeMagma α) → ρ ⊢ s e₁ e₂ e₃ ≃ ρ ⊢ (e₁ e₂) (e₁ e₃)
-  k_eval : {ρ : Bwd α} → {e₁ e₂ : FreeMagma α} → {a : α} → ρ ⊢ e₁ ⇓ a → ρ ⊢ e₂ ↓ → ρ ⊢ k e₁ e₂ ⇓ a
-  i_eval : {ρ : Bwd α} → {e : FreeMagma α} → {a : α} → ρ ⊢ e ⇓ a → ρ ⊢ i e ⇓ a
+  s_eval : (ρ : Bwd α) → (e₁ e₂ e₃ : FreeMagma α) → ρ ⊢ s e₁ e₂ e₃ ≃ ρ ⊢ (e₁ e₃) (e₂ e₃)
+  k_eval : (ρ : Bwd α) → (e₁ e₂ : FreeMagma α) → ρ ⊢ e₂ ↓ → ρ ⊢ k e₁ e₂ ≃ ρ ⊢ e₁
+  i_eval : (ρ : Bwd α) → (e : FreeMagma α) → ρ ⊢ i e ≃ ρ ⊢ e
 
 namespace SKI
 
@@ -103,12 +180,6 @@ theorem s_defined_1
   (e_defined : ρ ⊢ e ↓)
   : ρ ⊢ A.s e ↓ :=
   PAS.ap_left_defined (s_defined_2 e_defined (PAS.const_defined ρ k))
-
-theorem i_eval_inv
-  [A : SKI α]
-  {ρ : Bwd α} {e : FreeMagma α} {a : α}
-  (h : ρ ⊢ A.i e ⇓ a)
-  : ρ ⊢ e ⇓ a := by sorry
 
 @[simp] def abs [SKI α] : FreeMagma α → FreeMagma α
 | .var 0 => .const i
@@ -123,7 +194,7 @@ def abs_defined [SKI α] (ρ : Bwd α) (e : FreeMagma α) (h : e.fv ≤ ρ.lengt
     simp
     apply PAS.ap_defined
     · apply PAS.const_eval
-    · apply PAS.var_eval ρ ⟨ n , Nat.le_of_succ_le_succ h ⟩
+    · apply PAS.var_get_eval ρ ⟨ n , Nat.le_of_succ_le_succ h ⟩
     · apply SKI.k_defined
       apply PAS.const_defined
   | .const a =>
@@ -145,30 +216,62 @@ def abs_refines_le [SKI α] (ρ : Bwd α) (a : α) (e : FreeMagma α) : ρ ⊢ $
   intros v v_eval
   match e with
   | .var 0 =>
-    simp at v_eval
-    have cool : (ρ :# a) ⊢ $(FreeMagma.var 0) ⇓ a := PAS.var_eval (ρ :# a) ⟨ 0 , by simp ⟩
-    have cooler : ρ ⊢ a ⇓ v := by
-      apply i_eval_inv
+    simp at *
+    have var_eval : (ρ :# a) ⊢ `(0) ⇓ a := PAS.var_zero_eval ρ a
+    have a_eval : ρ ⊢ a ⇓ v := (i_eval ρ (FreeMagma.const a)).1 v v_eval
+    rwa [←PAS.const_eval_eq ρ a v a_eval]
+  | .var (n+1) =>
+     simp at *
+     apply (PAS.var_succ_eval ρ a n).2
+     apply (SKI.k_eval ρ (.var n) (.const a) _).1
+     · exact v_eval
+     · apply PAS.const_defined
+  | .const b =>
+    simp at *
+    apply PAS.const_eval_stable
+    apply (SKI.k_eval ρ (.const b) (.const a) _).1
+    · exact v_eval
+    · apply PAS.const_defined ρ a
+  | .ap e₁ e₂ =>
+    simp at *
+    have ap_abs_eval : ρ ⊢ ($(abs e₁) a) ($(abs e₂) a) ⇓ v := by
+      apply (SKI.s_eval ρ (abs e₁) (abs e₂) (.const a)).1
       exact v_eval
-    rwa [←PAS.const_eval_eq ρ a v cooler]
-  | .var (n+1) => sorry
-  | .const a => sorry
-  | .ap e₁ e₂ => sorry
+    have ⟨ v₁ , v₁_eval ⟩ := PAS.ap_left_defined ⟨ v , ap_abs_eval ⟩
+    have ⟨ v₂ , v₂_eval ⟩ := PAS.ap_right_defined ⟨ v , ap_abs_eval ⟩
+
+    apply (PAS.ap_eval (ρ₂ := ρ) (abs_refines_le ρ a e₁ v₁ v₁_eval) (abs_refines_le ρ a e₂ v₂ v₂_eval)).2
+    apply (PAS.ap_eval v₁_eval v₂_eval).1
+    exact ap_abs_eval
+
+def abs_refines_ge [SKI α] (ρ : Bwd α) (a : α) (e : FreeMagma α) : (ρ :# a) ⊢ e ≤ ρ ⊢ $(abs e) a := by
+  intros v v_eval
+  match e with
+  | .var 0 =>
+    simp at *
+    have var_eval : (ρ :# a) ⊢ `(0) ⇓ a := PAS.var_zero_eval ρ a
+    apply (i_eval _ _).2
+    rw [PAS.eval_functional v_eval var_eval]
+    apply PAS.const_eval
+  | .var (n+1) =>
+    simp at *
+    apply (k_eval ρ (.var n) (.const a) _).2
+    · apply (PAS.var_succ_eval ρ a n).1
+      exact v_eval
+    · apply PAS.const_defined
+  | .const b =>
+    simp at *
+    apply (k_eval ρ (.const b) (.const a) _).2
+    · apply PAS.const_eval_stable
+      exact v_eval
+    · apply PAS.const_defined
+  | .ap e₁ e₂ =>
+    simp at *
+    have ⟨ v₁ , v₁_eval ⟩ := PAS.ap_left_defined ⟨ v , v_eval ⟩
+    have ⟨ v₂ , v₂_eval ⟩ := PAS.ap_right_defined ⟨ v , v_eval ⟩
+    apply (s_eval ρ (abs e₁) (abs e₂) (.const a)).2
+    apply (PAS.ap_eval (ρ₂ := ρ) (abs_refines_ge ρ a e₁ v₁ v₁_eval) (abs_refines_ge ρ a e₂ v₂ v₂_eval)).2
+    apply (PAS.ap_eval v₁_eval v₂_eval).1
+    exact v_eval
 
 end SKI
-    -- exists _
-    -- sorry
-    -- exact ⟨ _ , _ ⟩
-    -- -- have ⟨  ⟩
-    -- sorry
-    -- -- apply PAS.ap_defined
-    -- -- · sorry
-    -- -- · exact a₂_defined
-    -- -- · sorry
-    -- -- -- · apply PAS.ap_defined
-    -- -- --   · apply PAS.const_eval
-    -- -- --   · apply PAS.const_eval
-    -- -- --   · apply PAS.ap_defined
-    -- -- --     · sorry
-    -- -- --     · sorry
-    -- -- --     · sorry
